src/Lib/DWT/VSTder_write_TL.v
@@ -19,11 +19,17 @@ Proof. make_cs_preserve CompSpecs  VSTber_tlv_tag_serialize.CompSpecs. Defined.
 Instance Change2 : change_composite_env  VSTber_tlv_tag_serialize.CompSpecs CompSpecs.
 Proof. make_cs_preserve  VSTber_tlv_tag_serialize.CompSpecs CompSpecs. Defined.
 
+Instance Change3 : change_composite_env CompSpecs  VSTber_tlv_length_serialize.CompSpecs.
+Proof. make_cs_preserve CompSpecs VSTber_tlv_length_serialize.CompSpecs. Defined.
+
+Instance Change4 : change_composite_env  VSTber_tlv_length_serialize.CompSpecs CompSpecs.
+Proof. make_cs_preserve  VSTber_tlv_length_serialize.CompSpecs CompSpecs. Defined.
+
 Open Scope Z.
 
 Definition der_write_TL tag len size := 
   let (_, t) := ber_tlv_tag_serialize tag (Int.repr size) in
-  let (_, l) := ber_tlv_length_serialize len (Int.repr size) in
+  let (_, l) := ber_tlv_length_serialize len (Int.repr (size - t)) in
   if ((t =? -1) || (t >? 32))%bool 
   then -1
   else if l =? -1 
@@ -33,9 +39,15 @@ Definition der_write_TL tag len size :=
             then -1
             else s.
 
-
-Lemma tag_serialize_bounds : forall t l, 0 <= snd (ber_tlv_tag_serialize t l) <= 32.
+Lemma tag_serialize_bounds : forall t l, -1 <= snd (ber_tlv_tag_serialize t l) <= 6.
       { unfold ber_tlv_tag_serialize.
+        intros.
+        cbn.
+        repeat break_if; autorewrite with norm; try nia. } 
+Qed.
+
+Lemma length_serialize_bounds : forall t l, -1 <= snd (ber_tlv_length_serialize t l) <= 6.
+      { unfold ber_tlv_length_serialize.
         intros.
         cbn.
         repeat break_if; autorewrite with norm; try nia. } 
@@ -125,7 +137,7 @@ Proof.
       assert (z = -1) as Z. 
       {  unfold ber_tlv_tag_serialize in *.
             break_if;
-              rewrite_if_b; admit. (* SPEC *) }
+              rewrite_if_b; auto. }
       break_if; try congruence.
       forward_if.
       repeat forward.
@@ -152,65 +164,158 @@ Proof.
            (force_val
          (sem_cast_i2bool
             (Val.of_bool
-               (Int.repr 32 < Int.repr 
-                                (snd (ber_tlv_tag_serialize tag (Int.repr 32))))%int)))))). 
+               (Int.repr 32 
+                < Int.repr 
+                    (snd (ber_tlv_tag_serialize tag (Int.repr 32))))%int)))))). 
       1-2: repeat forward;
            entailer!;
            rewrite_if_b;
            auto;
            break_if; entailer!. 
-      rewrite if_false.
-      forward_if.
-      repeat forward.
-      normalize in H0.
-      eapply typed_true_of_bool in H0.
-      clear H1.
-      unfold Int.lt in H0.
-      destruct zlt; try congruence.
-      do 2 rewrite Int.signed_repr in l; try rep_omega.
-      normalize in H0.
-      eapply typed_false_of_bool in H0.
-      unfold Int.lt in H0.
-      destruct zlt; try congruence.
-      do 2 rewrite Int.signed_repr in g; try rep_omega.
-      normalize.
-      rewrite if_false.
-      repeat forward.
-      normalize.
-      forward_if (temp _t'4 (Vint (Int.repr (32 - z)))); try congruence.
-      repeat forward.
-      entailer!. 
-      discriminate.
-      forward_call (len, b, (i + Ptrofs.repr z)%ptrofs, (32 - z), (32 - z)).
-      entailer!.
-      normalize.
-    (* unfold ber_tlv_tag_serialize.
-      destruct (30 >=? Int.unsigned (tag >>u Int.repr 2)) eqn: Z.
-      repeat rewrite_if_b.
-      entailer!.
-      admit. (* true *)
-      repeat rewrite_if_b.
-      entailer!.
-      admit. (* true *)
-      normalize.
-      autorewrite with norm.
-      repeat split; try rep_omega.
-      rewrite Int.unsigned_repr; try rep_omega.
-      (* need two buffers, each size 32 *)
-      admit.
-      admit. (* true *)
-      repeat forward.
-      forward_if.
-      repeat forward.
-      entailer!.
-      unfold der_write_TL.
-      repeat break_let.
-      simpl in H0.
-      inversion H0.
-      cbn in H.
-      cbn in H1.
-      admit.
-      entailer!. *)
+      break_if.
+      * assert (z = -1) as Z. 
+      { eapply repr_inj_signed;
+           try rep_omega; auto. }
+        forward_if; try discriminate.
+        forward.
+        entailer!.
+        unfold der_write_TL.
+        repeat break_let.     
+        cbn in Z. subst.
+        do 2 f_equal. 
+        break_if.
+        entailer!.
+        admit. (* can be singleton  - fix forward_if *)
+      *  assert (z <> -1) as Z. 
+        { eapply repr_neq_e. auto. }
+        forward_if.
+        repeat forward.
+        normalize in H0.
+        eapply typed_true_of_bool in H0.
+        clear H1.
+        unfold Int.lt in H0.
+        destruct zlt; try congruence.
+        do 2 rewrite Int.signed_repr in l; try rep_omega.
+        normalize in H0.
+        eapply typed_false_of_bool in H0.
+        unfold Int.lt in H0.
+        destruct zlt; try congruence.
+        do 2 rewrite Int.signed_repr in g; try rep_omega.
+        normalize.
+        rewrite if_false.
+        repeat forward.
+        normalize.
+        forward_if (temp _t'4 (Vint (Int.repr (32 - z)))); try congruence.
+        repeat forward.
+        entailer!. 
+        discriminate.
+        remember (fst (ber_tlv_tag_serialize tag (Int.repr 32))) as ls.         
+        erewrite data_at_app_gen 
+          with (j1 := z)
+               (j2 := 32 - z)
+               (ls1 := map Vint ls)
+               (ls2 := (default_val (tarray tuchar (32 - z))));
+          (autorewrite with sublist list norm; try rep_omega; auto).
+        forward_call (len, b, (i + Ptrofs.repr z)%ptrofs, (32 - z), (32 - z)).
+        unfold Frame.
+        instantiate
+          (1 := [valid_pointer cb;  data_at_ Tsh enc_key_s app_key;
+          data_at Tsh (tarray tuchar z) (map Vint ls) (Vptr b i)]). 
+        unfold fold_right_sepcon.
+        entailer!.
+        repeat split; try rep_omega.
+        1-2: ptrofs_compute_add_mul; try rep_omega.
+        repeat forward.
+        forward_if.
+         ** repeat forward.
+            entailer!.
+            unfold der_write_TL.
+            repeat break_let.
+            cbn in *.
+            do 2 f_equal.
+            replace ((z =? -1) || (z >? 32))%bool with false.
+            assert ((snd (ber_tlv_length_serialize len (Int.repr (32 - z)))) = z0) as B.
+            { unfold snd.
+              break_let.
+              auto.
+              inversion Heqp0.
+              auto. }
+            rewrite B in *.
+            pose proof (length_serialize_bounds len (Int.repr (32 - z))) as L.
+            assert (z0 = -1) as Z0. 
+            { eapply repr_inj_signed;
+                try rep_omega; auto. }
+            rewrite Z0.
+            auto.
+            symmetry.
+            eapply orb_false_intro;
+            Zbool_to_Prop; try nia.
+            erewrite Z.gtb_ltb.
+            Zbool_to_Prop. nia.
+            remember (snd (ber_tlv_tag_serialize tag (Int.repr 32))) as z.
+            remember (fst (ber_tlv_tag_serialize tag (Int.repr 32))) as ls.
+            break_let.
+            break_if. 
+            admit. (* fix SPE spec *)
+            admit.
+         ** repeat forward.
+            forward_if.
+            *** forward.
+                entailer!.
+                unfold der_write_TL.
+                repeat break_let.
+                cbn in *.
+                do 2 f_equal.
+                replace ((z =? -1) || (z >? 32))%bool with false.
+                assert ((snd (ber_tlv_length_serialize len (Int.repr (32 - z)))) = z0) as B.
+                { unfold snd.
+                  break_let.
+                  auto.
+                  inversion Heqp0.
+                  auto. }
+                rewrite B in *.
+                pose proof (length_serialize_bounds len (Int.repr (32 - z))) as L.
+                assert (z0 <> -1) as Z0. 
+                 { eapply repr_neq_e. auto. }
+                replace (z0 =? -1) with false.
+                replace (z0 + z >? 32) with true.
+                auto.
+                symmetry.
+                erewrite Z.gtb_ltb.
+                Zbool_to_Prop; try rep_omega.
+                rewrite Int.unsigned_repr in *; try rep_omega.
+                symmetry.
+                Zbool_to_Prop. nia.
+                symmetry.
+                eapply orb_false_intro;
+                  Zbool_to_Prop; try nia.
+                erewrite Z.gtb_ltb.
+                Zbool_to_Prop. nia.
+
+                remember (snd (ber_tlv_tag_serialize tag (Int.repr 32))) as z.
+                remember (fst (ber_tlv_tag_serialize tag (Int.repr 32))) as ls.
+                break_let.
+                break_if. 
+                admit. (* fix SEP spec *)
+                admit.
+            *** forward_if True; try congruence.
+                -- forward_if True.
+                ++
+                (* store - add to spec *)
+                admit.
+                ++
+                forward.
+                entailer!.
+                ++ 
+                (* forward call *)
+                admit.
+                --
+                forward.
+                entailer!.
+                do 2 f_equal.
+                admit. (* spec proof *)
+                admit. (* changes in memory from serialize tag and length *)
+     ** admit. (* add lemma *)
 Admitted.
-   
-        
+
+
